Source/DafnyCore/Compilers/Dafny/DAM.dfy
@@ -23,52 +23,186 @@ class Ptr<A> {
   }
 }
 
+type Var = string
+type Field = string
+
+//module Typing {
+datatype Pos =
+  Unit
+| Bool
+| Int
+| Thunk(Neg)
+| Ref(Pos)
+| Stack(Neg)
+
+datatype Neg =
+  Value(Pos)
+| Function(dom: Pos, cod: Neg)
+| Record(fields: map<Field, Neg>)
+
+type Context = map<Var, Pos>
+
+// Hamza-Voirol-Kuncak trick: annotate terms just enough so that ostensible checking terms synthesize
+
+function SynthPos(g: Context, e: Expr): Option<Pos> {
+    match e
+    case Var(x)   => if x in g then Some(g[x]) else None
+    case Unit     => Some(Pos.Unit)
+    case Bool(_)  => Some(Pos.Bool)
+    case Int(_)   => Some(Pos.Int)
+    case Thunk(s) => (
+        match SynthNeg(g, s)
+        case Some(t) => Some(Pos.Thunk(t))
+        case _       => None
+    )
+    case Ref(p)   => Some(Pos.Int)
+}
+
+predicate CheckPos(g: Context, e: Expr, t: Pos) {
+    SynthPos(g, e) == Some(t)
+}
+
+predicate CheckNeg(g: Context, s: Stmt, t: Neg) {
+    SynthNeg(g, s) == Some(t)
+}
+
+function SynthNeg(g: Context, s: Stmt): Option<Neg> decreases s {
+    match s
+    case Pure(e) => (
+        match SynthPos(g, e)
+        case Some(t) => Some(Neg.Value(t))
+        case _       => None
+    )
+    
+    case Bind(lhs, var_, rhs) => (
+        match SynthNeg(g, lhs)
+        case Some(Value(t)) => SynthNeg(g[var_ := t], rhs)
+        case _              => None
+    )
+    
+    /*case Ite(guard, then_, else_) => (
+        :- CheckPos(guard, Pos.Bool);
+        var t :- SynthNeg(g, then_, t);
+        if CheckNeg(g, else_, t) then Some(t) else None
+    )*/
+
+    case Func(bound, dom, body) => (
+        var cod :- SynthNeg(g[bound := dom], body);
+        Some(Function(dom, cod))
+    )
+
+    case Call(func, arg) => (
+        match SynthNeg(g, func)
+        case Some(Function(dom, cod)) => (
+            if CheckPos(g, arg, dom) then Some(cod) else None
+        )
+        case _ => None
+    )
+    
+    case Force(expr) => (
+        match SynthPos(g, expr)
+        case Some(Thunk(t)) => Some(t)
+        case _              => None
+    )
+
+    case Print(expr, next) => (
+        match SynthPos(g, expr)
+        case Some(_) => SynthNeg(g, next)
+        case _       => None
+    )
+
+    /*case Record(fields) => (
+        for i := 0 to  {
+            match SynthNeg(g, fields[i])
+            case Some() => 
+            case None   => return None;
+        }
+    )*/
+
+    case Select(record, field) => (
+        match SynthNeg(g, record)
+        case Some(Record(fields)) =>
+            if field in fields then Some(fields[field]) else None
+        case _ => None
+    )
+
+    case _ => None
+}
+
+//}
+
 datatype Expr =
 // G, x : A+ |- x : A+
-  Var(string)
+  Var(Var)
+| Unit
 // G |- true/false : Bool
 | Bool(bool)
-| Int(int)
+| Int(int) 
 // TODO: variant types
 | Thunk(Stmt)
 | Ref(Ptr<Val>)
 
-// G |- e : D and D |- V : A+ ~> G |- V 
 //type Heap = set<Ptr<Stmt>>
 
 datatype Stmt =
-// Intro & Elim for Up(A+)
+// Intro & Elim for expressions
   Pure(Expr)
-| Bind(lhs: Stmt, var_: string, rhs: Stmt)
+| Bind(lhs: Stmt, var_: Var, rhs: Stmt)
 // Elim for bools
 | Ite(guard: Expr, then_: Stmt, else_: Stmt)
 // Intro & Elim for arrows
-| Func(bound: string, body: Stmt)
+| Func(bound: Var, dom: Pos, body: Stmt)
 | Call(func: Stmt, arg: Expr)
 // Intro & Elim for objects/records
 | Record(fields: map<string, Stmt>)
-| Select(obj: Stmt, field: string)
+| Select(record: Stmt, field: Field)
 // Elim for thunks
 | Force(Expr)
 // Elims for refs
-| Read(ref: Expr, var_: string, cont: Stmt)
-| Write(l: Expr, r: Expr, cont: Stmt)
+| Read(ref: Expr, var_: Var, cont: Stmt)
+| Write(lvalue: Expr, rvalue: Expr, next: Stmt)
+// Print
+| Print(Expr, next: Stmt)
+// Recursion
+| Rec(bound: Var, body: Stmt)
+// Let-current-stack (letcc, basically) and throw
+| LetCS(bound: Var, body: Stmt)
+| Throw(stack: Expr, init: Stmt)
 {
     // TODO calculate Heap of a comp
 }
 
+// Let-bindings
+function Let(lhs: Expr, var_ : string, ty: Pos, rhs: Stmt): Stmt
+    { Stmt.Call(Func(var_, ty, rhs), lhs) }
+
+/** Guarded commands / imperative substrate of Dafny */
+function Then(lhs: Stmt, rhs: Stmt): Stmt
+    { Stmt.Bind(lhs, "_", rhs) }
+
+function Skip(): Stmt
+    { Pure(Expr.Unit) }
+
+function While(guard: Stmt, body: Stmt, next: Stmt): Stmt {
+    Rec("while", Stmt.Bind(guard, "if",
+        Ite(Var("if"), Then(body, Force(Var("while"))), next)))
+}
+
 // G |- (e, v) : A iff exists D. G |- e : D and D |- V : A
 datatype Val =
-  Bool(bool)
+  Unit
+| Bool(bool)
 | Int(int)
 | Thunk(Env, Stmt)
 | Ref(Ptr<Val>)
+| Stack(Env, Stack)
+
 // G |- e : D iff for all x : A in D, G |- e[x] : A
 type Env = map<string, Val>
 
-// 
+// Stack frames (one for each negative type elimination)
 datatype Frame =
-  Bind(var_: string, rhs: Stmt)
+  Bind(var_: Var, rhs: Stmt)
 | Call(arg: Expr)
 | Select(field: string)
 
@@ -93,6 +227,7 @@ function Eval(env: Env, expr: Expr): Val {
         // Type soundness will discharge this assumption
         assume {:axiom} x in env;
         env[x]
+    case Unit     => Val.Unit
     case Bool(b)  => Val.Bool(b)
     case Int(i)   => Val.Int(i)
     // The Felleisen-Friedman trick: delay
@@ -101,10 +236,9 @@ function Eval(env: Env, expr: Expr): Val {
     case Ref(ptr) => Val.Ref(ptr)
 }
 
-// This function either steps the current state or tells you that it's terminal/stuck
+// Small-step semantics
 // Type soundness = well-typed configs don't get stuck!
 // TODO: replace * with Heap of state
-// TODO: shouldn't stuck be auto-propagated?
 function Step(state: In): Out reads * {
     var (env, comp, stack) := state;
     match comp
@@ -115,7 +249,7 @@ function Step(state: In): Out reads * {
         match stack.Pop()
         case Some((Bind(var_, rhs), stack)) =>
             Next((env[var_ := Eval(env, expr)], rhs, stack))
-        
+
         case Some(_) => Stuck
         case None    => Terminal(Eval(env, expr))
     )
@@ -123,7 +257,7 @@ function Step(state: In): Out reads * {
     case Call(func, arg) =>
         Next((env, func, Push(Frame.Call(arg), stack)))
     
-    case Func(bound, body) => (
+    case Func(bound, _, body) => (
         match stack.Pop()
         case Some((Call(arg), stack)) =>
             Next((env[bound := Eval(env, arg)], body, stack))
@@ -138,7 +272,10 @@ function Step(state: In): Out reads * {
     case Record(fields) => (
         match stack.Pop()
         case Some((Select(field), stack)) =>
-            Next((env, fields[field], stack))
+            if field in fields then
+                Next((env, fields[field], stack))
+            else
+                Stuck
         
         case Some(_) => Stuck
         case None    => Terminal(Val.Thunk(env, comp))
@@ -155,9 +292,8 @@ function Step(state: In): Out reads * {
     // Lexical scope restores the env of the closure
     case Force(thunk) => (
         match Eval(env, thunk)
-        case Thunk(env, c) => Next((env, c, stack))
-        
-        case _        => Stuck
+        case Thunk(env, comp) => Next((env, comp, stack))
+        case _             => Stuck
     )
     
     case Read(ref, var_, cont) => (
@@ -166,15 +302,32 @@ function Step(state: In): Out reads * {
         case _        => Stuck
     )
 
-    case Write(lhs, rhs, cont) => (
-        match Eval(env, lhs)
+    case Write(lval, rval, next) => (
+        match Eval(env, lval)
         case Ref(ptr) =>
-            (/*ptr.deref := Eval(env, rhs);*/ Next((env, cont, stack)))
+            (/*ptr.deref := Eval(env, rval);*/ Next((env, next, stack)))
         case _        => Stuck
+    )
+
+    case Print(expr, next) =>
+        (/*print Eval(env, expr), "\n";*/ Next((env, next, stack)))
+
+    case Rec(self, body) =>
+        Next((env[self := Val.Thunk(env, comp)], body, stack))
+
+    case LetCS(bound, body) =>
+        Next((env[bound := Val.Stack(env, stack)], body, stack))
+    
+    case Throw(stack, init) => (
+        match Eval(env, stack)
+        case Stack(env, stack) => Next((env, init, stack))
+        case _                 => Stuck
     )
 }
 
-// Iterates step
+//codatatype Trace = Next(In, Trace) | Stuck | Terminal(Val)
+
+// Big-step semantics coinductively iterates the small-step
 method Run(s: In) decreases * {
     print("\n");
     match Step(s)
@@ -185,9 +338,6 @@ method Run(s: In) decreases * {
 // Initial configuration
 function Initial(comp: Stmt): In
     { (map[], comp, Empty) }
-
-function Let(lhs: Expr, var_ : string, rhs: Stmt): Stmt
-    { Stmt.Call(Func(var_, rhs), lhs) }
 
 method Main() decreases * {
     Run(Initial(
@@ -202,23 +352,17 @@ method Main() decreases * {
         )
     ));
     // Verifies that lexical scope works
-    var fc := Expr.Thunk(Func("y", Pure(Var("x"))));
+    var fc := Expr.Thunk(Func("y", Pos.Int, Pure(Var("x"))));
     var fv := Force(Var("f"));
     var x1 := Expr.Int(1);
     var x2 := Expr.Int(2);
     var z  := Expr.Int(0);
     Run(Initial(
-        Let(x1, "x",
-        Let(fc, "f",
-        Let(x2, "x",
+        Let(x1, "x", Pos.Int,
+        Let(fc, "f", Pos.Int,
+        Let(x2, "x", Pos.Int,
         Stmt.Call(fv, z))))
     ));
 }
 
-
-
-/*function While(guard: Stmt, body: Stmt) {
-  Call(Fix(Lambda("while",
-    Ite(guard, Then(body, "while"), ))), ());
-}*/
 }
