Source/DafnyCore/Compilers/ResolvedDesugaredExecutableDafny/Dafny-compiler-fdafny.dfy
@@ -6,10 +6,16 @@ module {:extern "ResolvedDesugaredExecutableDafnyPlugin"} ResolvedDesugaredExecu
 
   class COMP {
 
-    static method Compile(p: seq<Module>) returns (s: string) {
-      var st := EmitDAM(p);
-      print st;
-      print "\n";
+    static method Compile(p: seq<Module>) returns (s: string) decreases * {
+      //print(p);
+      for i := 0 to |p| {
+        var m := EmitModule(p[i]);
+        var t := EmitModuleType(p[i]);
+        print m;
+        print "\n\n";
+        print t;
+        print "\n\n";
+      }
 
       s := PrettyPrinter.PrettyPrint(p);
     }
@@ -18,30 +24,108 @@ module {:extern "ResolvedDesugaredExecutableDafnyPlugin"} ResolvedDesugaredExecu
       s := "";
     }
 
-    // Modules are just classes, really
-    static method EmitModule(m: Module) returns (s: DAM.Stmt) {
-      s := EmitClass(Class(m.name, "", [], [], [], []));
+    static method PolarizePos(t: Type) returns (p: DAM.Pos) {
+      match t
+      case Primitive(Int)  => p := DAM.Pos.Int;
+      case Primitive(Bool) => p := DAM.Pos.Bool;
+      case _ => UnsupportedFeature.Throw(); p := DAM.Pos.Unit;
     }
 
-    // TODO: Classes/traits are implemented as fixed points of records: Fix(\this. {field1 = ..., fieldn = ...})
+    static method EmitModuleType(m: Module) returns (t: DAM.Neg) {
+      var members := map[];
+      for i := 0 to |m.body| {
+        match m.body[i]
+        case Module(m) =>
+          var tm := EmitModuleType(m);
+          members := members[m.name := tm];
+        case Class(c) =>
+          var tc := EmitClassType(c);
+          members := members[c.name := tc];
+        case _ => continue;
+      }
+      t := DAM.Neg.Record(members);
+    }
+
+    static method EmitClassType(c: Class) returns (t: DAM.Neg) {
+      var members := map[];
+      for i := 0 to |c.body| {
+        match c.body[i]
+        case Method(m) =>
+          var tm := EmitMethodType(m);
+          members := members[m.name := tm];
+      }
+      t := DAM.Neg.Record(members);
+    }
+
+    static method EmitMethodType(m: Method) returns (t: DAM.Neg) {
+      t := DAM.Neg.Value(DAM.Pos.Unit);
+      for i := 0 to |m.params| {
+        match m.params[|m.params| - i - 1]
+        case Formal(_, dom) =>
+          var dom := PolarizePos(dom);
+          t := DAM.Neg.Function(dom, t);
+      }
+      // TODO out parameters
+    }
+
+    // Modules are just records
+    static method EmitModule(m: Module) returns (s: DAM.Stmt) decreases * {
+      var members := map[];
+      for i := 0 to |m.body| {
+        match m.body[i]
+        case Module(m) =>
+          var mod := EmitModule(m);
+          members := members[m.name := mod];
+        case Class(c) =>
+          var cls := EmitClass(c);
+          members := members[c.name := cls];
+        // Types don't exist at the level of statements
+        case _ => continue;
+      }
+      s := DAM.Stmt.Record(members);
+    }
+
+    // TODO: Classes are fixed points of records: Fix(\this. {field1 = ..., fieldn = ...})
     // Methods are just functions
-    static method EmitClass(c: Class) returns (s: DAM.Stmt) {
+    static method EmitClass(c: Class) returns (s: DAM.Stmt) decreases * {
       var fields := map[];
       // TODO: normal fields turn into references
+      /*for i := 0 to |c.fields| {
+        match c.fields[i]
+        case Field(name, defaultValue) =>
+          fields := fields[name := DAM.Expr.Ref(new DAM.Ptr())];
+        case _ => UnsupportedFeature.Throw(); s := DAM.Skip();
+      }*/
       for i := 0 to |c.body| {
         match c.body[i]
         case Method(m) =>
           var meth := EmitMethod(m);
           fields := fields[m.name := meth];
       }
-      s := DAM.Record(fields);
+      s := DAM.Stmt.Record(fields);
     }
 
-    static method EmitMethod(m: Method) returns (s: DAM.Stmt) {
-      // TODO this is actually a lambda
-      s := EmitBlock(m.body);
+    static method EmitMethod(m: Method) returns (s: DAM.Stmt) decreases * {
+      // Label a point for early returns
+      var body := EmitBlock(m.body);
+      s := DAM.LetCS("return", body);
+      // Out parameters turn into input references
+      /*for i := 0 to |m.outVars| {
+        match m.outVars
+        case Ident(Ident(v)) =>
+        
+      }*/
+      // In parameters...also turn into input references
+      for i := 0 to |m.params| {
+        match m.params[|m.params| - i - 1]
+        case Formal(arg, dom) =>
+          var dom := PolarizePos(dom);
+          s := DAM.Func(arg, dom, s);
+      }
+      // Annotate the entire function to allow it to appear in a redex
     }
 
+    // Dafny expressions are actually DAM statements, since they are sensitive to evaluation order
     static method EmitExpr(e: Expression) returns (s: DAM.Stmt) {
       match e
       case Ident(v) => s := DAM.Pure(DAM.Var(v));
@@ -50,27 +134,77 @@ module {:extern "ResolvedDesugaredExecutableDafnyPlugin"} ResolvedDesugaredExecu
         var cond := EmitExpr(cond);
         var thn  := EmitExpr(thn);
         var els  := EmitExpr(els);
-        s := DAM.Stmt.Bind(cond, "_guard", DAM.Ite(DAM.Var("_guard"), thn, els));
-      case _ => s := DAM.Pure(DAM.Expr.Bool(true));
+        s := DAM.Stmt.Bind(cond, "if", DAM.Ite(DAM.Var("if"), thn, els));
+      case _ => UnsupportedFeature.Throw(); s := DAM.Skip();
     }
 
-    static method EmitStmt(s: Statement) returns (st: DAM.Stmt) {
-      match s
+    // Terminates by multiset ordering on block
+    static method EmitBlock(block: seq<Statement>) returns (st: DAM.Stmt) decreases * {
+      if (|block| <= 0) { return DAM.Skip(); }
+      var next := block[1..];
+      match block[0]
+
       case If(cond, thn, els) =>
         var cond := EmitExpr(cond);
         var thn  := EmitBlock(thn);
         var els  := EmitBlock(els);
-        st := DAM.Stmt.Bind(cond, "_guard", DAM.Ite(DAM.Var("_guard"), thn, els));
-      case _ => st := DAM.Pure(DAM.Expr.Bool(true));
+        var next := EmitBlock(next);
+        st := DAM.Then(DAM.Stmt.Bind(cond, "if", DAM.Ite(DAM.Var("if"), thn, els)), next);
+      
+      case While(guard, body) =>
+        var guard := EmitExpr(guard);
+        var body := EmitBlock(body);
+        var next := EmitBlock(next);
+        st := DAM.While(guard, body, next);
+      
+      // Breaks, returns, and halts drop the rest of the block
+      case Break(lab) => {
+        match lab
+        case Some(lab) =>
+          st := DAM.Throw(DAM.Var(lab), DAM.Skip());
+        case None => UnsupportedFeature.Throw(); st := DAM.Skip();
+      }
+
+      case EarlyReturn() =>
+        st := DAM.Throw(DAM.Var("return"), DAM.Skip());
+      
+      case Return(expr) =>
+        var ret := EmitExpr(expr);
+        st := DAM.Throw(DAM.Var("return"), ret);
+
+      case Labeled(lab, stmt) =>
+        var block := EmitBlock(stmt + next);
+        st := DAM.LetCS(lab, block);
+      
+      case Assign(lhs, rhs) =>
+        var lhs := EmitLval(lhs);
+        var rhs := EmitExpr(rhs);
+        var next := EmitBlock(next);
+        st := DAM.Stmt.Bind(lhs, "var",
+              DAM.Stmt.Bind(rhs, "rhs",
+                DAM.Write(DAM.Var("rhs"), DAM.Var("var"), next)));
+      
+      /*case Call(obj, meth, _, args, outs) =>
+        var obj := EmitExpr(obj);
+        s := DAM.Select(obj, meth);
+        for i := 0 to |args| {
+          var arg := EmitExpr(args[i]);
+          s := DAM.Stmt.Bind(arg, "arg" + i,
+            DAM.Stmt.Call(s, DAM.Var("arg" + i)));
+        } */
+      
+      case Print(expr) =>
+        var arg := EmitExpr(expr);
+        var next := EmitBlock(next);
+        st := DAM.Stmt.Bind(arg, "var", DAM.Print(DAM.Var("var"), next));
+      
+      case _ => UnsupportedFeature.Throw(); st := DAM.Skip();
     }
 
-    static method EmitBlock(b: seq<Statement>) returns (s: DAM.Stmt) {
-      s := DAM.Pure(DAM.Expr.Bool(true));
-      if (|b| > 0) {
-        var first := EmitStmt(b[0]);
-        var rest  := EmitBlock(b[1..]);
-        s := DAM.Stmt.Bind(first, "_", rest);
-      }
+    static method EmitLval(lv: AssignLhs) returns (s: DAM.Stmt) {
+      match lv
+      case Ident(Ident(v)) => s := DAM.Pure(DAM.Var(v));
+      case _        => s := DAM.Skip();
     }
   }
 }
